Lean4Lean/Theory/Typing/InductiveLemmas.lean
@@ -1,10 +1,11 @@
 import Std
 import Lean4Lean.Theory.Typing.Lemmas
 import Lean4Lean.Theory.Typing.Env
+import Lean4Lean.Theory.Inductive.Lemmas
 
 namespace Lean4Lean
 namespace VEnv
 
 theorem addInduct_WF (henv : Ordered env) (hdecl : decl.WF env)
     (henv' : addInduct' env decl = some env') : Ordered env' :=
-  sorry
+  VInductDecl'.addInduct'_ordered_final henv hdecl henv'
